The bug was that inner loop counter j wasn't being reset. Might need lemmas to convince the recLCS post condition?

dp/lcs.dfy
@@ -3,11 +3,13 @@
  * 1. https://en.wikipedia.org/wiki/Longest_common_subsequence_problem#Worked_example
  */
 
+include "util.dfy"
+
 predicate rowColInitializedMatrix(a: array2<nat>)
 reads a
 {
-    forall i, j :: ((0 <= i < a.Length0 && 0 <= j < a.Length1) 
-                    && ((i == 0 && 0 <= j < a.Length1) || (j == 0 && 0 <= i < a.Length0))) 
+    forall i, j :: (0 <= i < a.Length0 && 0 <= j < a.Length1) 
+                    ==> ((i == 0 && 0 <= j < a.Length1) || (j == 0 && 0 <= i < a.Length0)) 
                     ==> a[i, j] == 0 
 }
 
@@ -42,22 +44,30 @@ modifies lcsMatrix
 requires 0 < lcsMatrix.Length0 == |s1| && 0 < lcsMatrix.Length1 == |s2|
 requires rowColInitializedMatrix(lcsMatrix)
 requires leftPaddedDimMatrix(s1, s2, lcsMatrix)
+ensures rowColInitializedMatrix(lcsMatrix)
 ensures lcsLen == recLCS(s1, s2, |s1|-1, |s2|-1)
 {
     var rowLen, colLen := |s1|, |s2|;
-    var i, j := 1, 1;
+    var i, j :=  1, 1;
 
     while i < rowLen
     decreases rowLen - i
     invariant 1 <= i <= rowLen
-    invariant 1 <= j <= colLen
+    invariant forall x :: 0 <= x < |s2| ==> lcsMatrix[0, x] == 0
+    invariant forall x :: 0 <= x < |s1| ==> lcsMatrix[x, 0] == 0
     {
+        j := 1;
+
         while j < colLen
         decreases colLen - j
         invariant 1 <= j <= colLen
+        invariant forall x :: 0 <= x < |s2| ==> lcsMatrix[0, x] == 0
+        invariant forall x :: 0 <= x < |s1| ==> lcsMatrix[x, 0] == 0
         {
             if s1[i] == s2[j]
-                { lcsMatrix[i, j] := 1 + lcsMatrix[i-1, j-1]; }
+                { 
+                    lcsMatrix[i, j] := 1 + lcsMatrix[i-1, j-1]; 
+                }
             else
                 { 
                     lcsMatrix[i, j] := if lcsMatrix[i, j-1] > lcsMatrix[i-1, j]
@@ -73,19 +83,22 @@ ensures lcsLen == recLCS(s1, s2, |s1|-1, |s2|-1)
     lcsLen := lcsMatrix[|s1|-1, |s2|-1];
 }
 
-method main() returns (x: nat)
+method Main() 
 {
-    var s1, s2 := "\0", "\0";
-    var a := new nat[|s1|, |s2|];
+    var s1, s2 := "\0AGCAT", "\0GAC";
+    var a := new nat[|s2|, |s1|];
 
-    forall i | 0 <= i < |s1| {
+    forall i | 0 <= i < |s2| {
         a[i, 0] := 0; 
     }
 
-    forall j | 0 <= j < |s2| {
+    forall j | 0 <= j < |s1| {
         a[0, j] := 0; 
     }
 
-    x := dpLCS(s1, s2, a); 
-    assert x == 0;
+
+    var x := dpLCS(s2, s1, a); 
+    //assert x == 2;
+
+    Util.printMatrix(a);
 }
